Limit function calls to earlier definition context.

Minimp.v
@@ -44,8 +44,12 @@ Record class : Set := mk_class {
 
 Definition program : Type := list class.
 
-Definition find_class (n: ident) : program -> option class :=
-  List.find (fun c=> ident_eqb c.(c_name) n).
+Definition find_class (n: ident) : program -> option (class * list class) :=
+  fix find (p: program) :=
+    match p with
+    | [] => None
+    | c :: p' => if ident_eqb c.(c_name) n then Some (c, p') else find p'
+    end.
 
 (** ** Semantics *)
 
@@ -101,249 +105,184 @@ Proof.
     ( injection Hv2; trivial ) || apply Hv2.
 Qed.
 
-Section stmt_eval.
-  Variable prog : program.
+Inductive stmt_eval :
+  program -> memoryEnv -> constEnv -> stmt -> memoryEnv * constEnv -> Prop :=
+| Iassign:
+    forall prog menv env x e v env',
+      exp_eval menv env e v ->
+      PM.add x v env = env' ->
+      stmt_eval prog menv env (Assign x e) (menv, env')
+| Iassignst:
+    forall prog menv env x e v menv',
+      exp_eval menv env e v ->
+      add_mem x v menv = menv' ->
+      stmt_eval prog menv env (AssignSt x e) (menv', env)
+| Istep:
+    forall prog menv env e v clsid o y menv' env' omenv omenv' rv,
+      find_obj o menv = Some(omenv) ->
+      exp_eval menv env e v ->
+      stmt_step_eval prog omenv clsid v omenv' rv ->
+      add_obj o omenv' menv = menv' ->
+      PM.add y rv env  = env' ->
+      stmt_eval prog menv env (Step_ap y clsid o e) (menv', env')
+| Ireset:
+    forall prog menv env o clsid omenv' menv',
+      stmt_reset_eval prog clsid omenv' ->
+      add_obj o omenv' menv = menv' ->
+      stmt_eval prog menv env (Reset_ap clsid o) (menv', env)
+| Icomp:
+    forall prog menv env a1 a2 env1 menv1 env2 menv2,
+      stmt_eval prog menv env a1 (menv1, env1) ->
+      stmt_eval prog menv1 env1 a2 (menv2, env2) ->
+      stmt_eval prog menv env (Comp a1 a2) (menv2, env2)
+| Iifte_true:
+    forall prog menv env b ifTrue ifFalse env' menv',
+      exp_eval menv env b (Cbool true) ->
+      stmt_eval prog menv env ifTrue (menv', env') ->
+      stmt_eval prog menv env (Ifte b ifTrue ifFalse) (menv', env')
+| Iifte_false:
+    forall prog menv env b ifTrue ifFalse env' menv',
+      exp_eval menv env b (Cbool false) ->
+      stmt_eval prog menv env ifFalse (menv', env') ->
+      stmt_eval prog menv env (Ifte b ifTrue ifFalse) (menv', env')
+| Iskip:
+    forall prog menv env,
+      stmt_eval prog menv env Skip (menv, env)
+with stmt_step_eval :
+       program -> memoryEnv -> ident -> const -> memoryEnv -> const -> Prop :=
+| Iestep:
+    forall prog menv clsid iv prog' menv' ov cls env',
+      find_class clsid prog = Some(cls, prog') ->
+      stmt_eval prog' menv (PM.add cls.(c_input) iv empty) cls.(c_step)
+                (menv', env') ->
+      PM.find cls.(c_output) env' = Some(ov) ->
+      stmt_step_eval prog menv clsid iv menv' ov
+with stmt_reset_eval : program -> ident -> memoryEnv -> Prop :=
+| Iereset:
+    forall prog clsid cls prog' menv' env',
+      find_class clsid prog = Some(cls, prog') ->
+      stmt_eval prog' mempty empty cls.(c_reset) (menv', env') ->
+      stmt_reset_eval prog clsid menv'.
 
-  (* (* version: menv, env as parameters *)
-  Inductive stmt_eval (menv: memoryEnv) (env: constEnv) :
-    stmt -> memoryEnv * constEnv -> Prop :=
-  | Iassign:
-      forall x e v env',
-        exp_eval menv env e v ->
-        PM.add x v env = env' ->
-        stmt_eval menv env (Assign x e) (menv, env')
-  | Iassignst:
-      forall x e v menv',
-        exp_eval menv env e v ->
-        add_mem x v menv = menv' ->
-        stmt_eval menv env (AssignSt x e) (menv', env)
-  | Istep:
-      forall e v clsid cls o y menv' env' omenv omenv' rv,
-        find_class clsid prog = Some(cls) ->
-        find_obj o menv = Some(omenv) ->
+Scheme stmt_eval_mult := Induction for stmt_eval Sort Prop
+with stmt_step_eval_mult := Induction for stmt_step_eval Sort Prop
+with stmt_reset_eval_mult := Induction for stmt_reset_eval Sort Prop.
 
-        exp_eval menv env e v ->
-        stmt_step_eval omenv (PM.add cls.(c_input) v empty) cls omenv' rv ->
-        add_obj o omenv' menv = menv' ->
-        PM.add y rv env  = env' ->
-        stmt_eval menv env (Step_ap y clsid o e) (menv', env')
-  | Ireset:
-      forall o clsid omenv' menv',
-        stmt_reset_eval mempty empty clsid omenv' ->
-        add_obj o omenv' menv = menv' ->
-        stmt_eval menv env (Reset_ap clsid o) (menv', env)
-  | Icomp:
-      forall a1 a2 env1 menv1 env2 menv2,
-        stmt_eval menv env a1 (menv1, env1) ->
-        stmt_eval menv1 env1 a2 (menv2, env2) ->
-        stmt_eval menv env (Comp a1 a2) (menv2, env2)
-  | Iifte_true:
-      forall b ifTrue ifFalse env' menv',
-        exp_eval menv env b (Cbool true) ->
-        stmt_eval menv env ifTrue (menv', env') ->
-        stmt_eval menv env (Ifte b ifTrue ifFalse) (menv', env')
-  | Iifte_false:
-      forall b ifTrue ifFalse env' menv',
-        exp_eval menv env b (Cbool false) ->
-        stmt_eval menv env ifFalse (menv', env') ->
-        stmt_eval menv env (Ifte b ifTrue ifFalse) (menv', env')
-  | Iskip:
-        stmt_eval menv env Skip (menv, env)
-  with stmt_step_eval (menv: memoryEnv) (env: constEnv) :
-         class -> memoryEnv -> const -> Prop :=
-  | Iestep:
-      forall ov cls menv' env',
-        stmt_eval menv env cls.(c_step) (menv', env') ->
-        PM.find cls.(c_output) env' = Some(ov) ->
-        stmt_step_eval menv env cls menv' ov
-  with stmt_reset_eval (menv: memoryEnv) (env: constEnv) :
-         ident -> memoryEnv -> Prop :=
-  | Iereset:
-      forall clsid cls menv' env',
-        find_class clsid prog = Some(cls) ->
-        stmt_eval menv env cls.(c_reset) (menv', env') ->
-        stmt_reset_eval menv env clsid menv'.
-   *)
+Inductive run :
+  program -> memoryEnv -> constEnv -> stmt -> nat ->
+  memoryEnv * constEnv -> Prop :=
+| Run_empty:
+    forall prog menvInit envInit stmt,
+      run prog menvInit envInit stmt 0 (menvInit, envInit)
+| Run_cons:
+    forall prog menvInit menvInter menvFinal
+           envInit envInter envFinal stmt n,
+      stmt_eval prog menvInit envInit stmt (menvInter, envInter) ->
+      run prog menvInter envInter stmt n (menvFinal, envFinal) ->
+      run prog menvInit envInit stmt (S n) (menvFinal, envFinal).
 
-  Inductive stmt_eval :
-    memoryEnv -> constEnv -> stmt -> memoryEnv * constEnv -> Prop :=
-  | Iassign:
-      forall menv env x e v env',
-        exp_eval menv env e v ->
-        PM.add x v env = env' ->
-        stmt_eval menv env (Assign x e) (menv, env')
-  | Iassignst:
-      forall menv env x e v menv',
-        exp_eval menv env e v ->
-        add_mem x v menv = menv' ->
-        stmt_eval menv env (AssignSt x e) (menv', env)
-  | Istep:
-      forall menv env e v clsid o y menv' env' omenv omenv' rv,
-        find_obj o menv = Some(omenv) ->
-        exp_eval menv env e v ->
-        stmt_step_eval omenv clsid v omenv' rv ->
-        add_obj o omenv' menv = menv' ->
-        PM.add y rv env  = env' ->
-        stmt_eval menv env (Step_ap y clsid o e) (menv', env')
-  | Ireset:
-      forall menv env o clsid omenv' menv',
-        stmt_reset_eval clsid omenv' ->
-        add_obj o omenv' menv = menv' ->
-        stmt_eval menv env (Reset_ap clsid o) (menv', env)
-  | Icomp:
-      forall menv env a1 a2 env1 menv1 env2 menv2,
-        stmt_eval menv env a1 (menv1, env1) ->
-        stmt_eval menv1 env1 a2 (menv2, env2) ->
-        stmt_eval menv env (Comp a1 a2) (menv2, env2)
-  | Iifte_true:
-      forall menv env b ifTrue ifFalse env' menv',
-        exp_eval menv env b (Cbool true) ->
-        stmt_eval menv env ifTrue (menv', env') ->
-        stmt_eval menv env (Ifte b ifTrue ifFalse) (menv', env')
-  | Iifte_false:
-      forall menv env b ifTrue ifFalse env' menv',
-        exp_eval menv env b (Cbool false) ->
-        stmt_eval menv env ifFalse (menv', env') ->
-        stmt_eval menv env (Ifte b ifTrue ifFalse) (menv', env')
-  | Iskip:
-      forall menv env,
-        stmt_eval menv env Skip (menv, env)
-  with stmt_step_eval :
-         memoryEnv -> ident -> const -> memoryEnv -> const -> Prop :=
-  | Iestep:
-      forall menv clsid iv menv' ov cls env',
-        find_class clsid prog = Some(cls) ->
-        stmt_eval menv (PM.add cls.(c_input) iv empty) cls.(c_step)
-                  (menv', env') ->
-        PM.find cls.(c_output) env' = Some(ov) ->
-        stmt_step_eval menv clsid iv menv' ov
-  with stmt_reset_eval : ident -> memoryEnv -> Prop :=
-  | Iereset:
-      forall clsid cls menv' env',
-        find_class clsid prog = Some(cls) ->
-        stmt_eval mempty empty cls.(c_reset) (menv', env') ->
-        stmt_reset_eval clsid menv'.
-
-  Scheme stmt_eval_mult := Induction for stmt_eval Sort Prop
-  with stmt_step_eval_mult := Induction for stmt_step_eval Sort Prop
-  with stmt_reset_eval_mult := Induction for stmt_reset_eval Sort Prop.
-
-  Inductive run :
-    memoryEnv -> constEnv -> stmt -> nat -> memoryEnv * constEnv -> Prop :=
-  | Run_empty:
-      forall menvInit envInit stmt,
-        run menvInit envInit stmt 0 (menvInit, envInit)
-  | Run_cons:
-      forall menvInit menvInter menvFinal
-             envInit envInter envFinal
-             stmt n,
-        stmt_eval menvInit envInit stmt (menvInter, envInter) ->
-        run menvInter envInter stmt n (menvFinal, envFinal) ->
-        run menvInit envInit stmt (S n) (menvFinal, envFinal).
-
-  Lemma stmt_eval_fold_left_shift:
-    forall A f (xs:list A) iacc menv env menv' env',
-      stmt_eval menv env
-                (List.fold_left (fun i x => Comp (f x) i) xs iacc)
-                (menv', env')
-      <->
-      exists menv'' env'',
-        stmt_eval menv env
-                  (List.fold_left (fun i x => Comp (f x) i) xs Skip)
-                  (menv'', env'')
-        /\
-        stmt_eval menv'' env'' iacc (menv', env').
-  Proof.
-    Hint Constructors stmt_eval.
-    induction xs.
-    - split; [ now eauto | ].
-      intro H; do 2 destruct H.
-      destruct H as [H0 H1].
-      inversion_clear H0; apply H1.
-    - intros.
-      split.
-      + intro H0.
-        apply IHxs in H0.
-        destruct H0 as [menv'' H0].
-        destruct H0 as [env'' H0].
-        destruct H0 as [H0 H1].
-        inversion_clear H1.
-        exists menv1. exists env1.
-        split; try apply IHxs; eauto.
-      + intros;
-        repeat progress
+Lemma stmt_eval_fold_left_shift:
+  forall A prog f (xs:list A) iacc menv env menv' env',
+    stmt_eval prog menv env
+              (List.fold_left (fun i x => Comp (f x) i) xs iacc)
+              (menv', env')
+    <->
+    exists menv'' env'',
+      stmt_eval prog menv env
+                (List.fold_left (fun i x => Comp (f x) i) xs Skip)
+                (menv'', env'')
+      /\
+      stmt_eval prog menv'' env'' iacc (menv', env').
+Proof.
+  Hint Constructors stmt_eval.
+  induction xs.
+  - split; [ now eauto | ].
+    intro H; do 2 destruct H.
+    destruct H as [H0 H1].
+    inversion_clear H0; apply H1.
+  - intros.
+    split.
+    + intro H0.
+      apply IHxs in H0.
+      destruct H0 as [menv'' H0].
+      destruct H0 as [env'' H0].
+      destruct H0 as [H0 H1].
+      inversion_clear H1.
+      exists menv1. exists env1.
+      split; try apply IHxs; eauto.
+    + intros;
+      repeat progress
              match goal with
              | H:exists _, _ |- _ => destruct H
              | H:_ /\ _ |- _ => destruct H
-             | H:stmt_eval _ _ (Comp _ Skip) _ |- _ => inversion_clear H
-             | H:stmt_eval _ _ Skip _ |- _ => inversion H; subst
-             | H:stmt_eval _ _ (List.fold_left _ _ _) _ |- _ => apply IHxs in H
+             | H:stmt_eval _ _ _ (Comp _ Skip) _ |- _ => inversion_clear H
+             | H:stmt_eval _ _ _ Skip _ |- _ => inversion H; subst
+             | H:stmt_eval _ _ _ (List.fold_left _ _ _) _ |- _ => apply IHxs in H
              | _ => eauto
              end.
-        apply IHxs; eauto.
-  Qed.
+      apply IHxs; eauto.
+Qed.
 
-  Lemma stmt_eval_det:
-    forall s menv env renv1 renv2,
-      stmt_eval menv env s renv1
-      -> stmt_eval menv env s renv2
-      -> renv1 = renv2.
-  Proof.
-    intros s menv env renv1 renv2 Hs1.
-    revert renv2.
-    induction Hs1 using stmt_eval_mult
-    with (P:=fun menv env s renv1 sev=>
-               forall renv2, stmt_eval menv env s renv2 -> renv1 = renv2)
-         (P0:=fun menv clsid v menv' rv ssev=>
-                forall menv'' rv', stmt_step_eval menv clsid v menv'' rv'
-                                   -> menv' = menv'' /\ rv = rv')
-         (P1:=fun i menv srev=>
-                forall menv', stmt_reset_eval i menv' -> menv = menv');
-      inversion_clear 1;
-      repeat progress match goal with
-      | Ht: exp_eval ?menv ?env ?e (Cbool true),
-        Hf: exp_eval ?menv ?env ?e (Cbool false) |- _ =>
-        pose proof (exp_eval_det _ _ _ _ _ Ht Hf) as Hneq; discriminate
-      | H1:exp_eval ?menv ?env ?e ?v1,
-        H2:exp_eval ?menv ?env ?e ?v2 |- _ =>
-        pose proof (exp_eval_det _ _ _ _ _ H1 H2) as Heq;
-          rewrite Heq in *; clear Heq H1 H2
-      | H1: PM.add ?x ?v ?env = ?env1,
-        H2: PM.add ?x ?v ?env = ?env2 |- _ =>
-        rewrite H1 in H2; rewrite H2 in *; clear H1 H2
-      | H1: add_mem ?x ?v ?menv = ?menv1,
-        H2: add_mem ?x ?v ?menv = ?menv2 |- _ =>
-        rewrite H1 in H2; rewrite H2 in *; clear H1 H2
-      | H1: find_obj ?o ?menv = Some ?omenv1,
-        H2: find_obj ?o ?menv = Some ?omenv2 |- _ =>
-        rewrite H1 in H2; injection H2; intro Heq; rewrite Heq in *;
-        clear H1 H2 Heq
-      | H1: find_class ?clsid ?prog = _,
-        H2: find_class ?clsid ?prog = _ |- _ =>
-        rewrite H1 in H2; injection H2;
-        intro Heq; rewrite Heq in *; clear H2 H2
-      | H1: PM.find ?x ?env = ?rv1,
-        H2: PM.find ?x ?env = ?rv2 |- _ =>
-        rewrite H1 in H2; injection H2; rewrite H2 in *; clear H1 H2
-      | Hs: stmt_step_eval ?omenv ?clsid ?v _ _,
-        IH: context[stmt_step_eval ?omenv ?clsid ?v _ _ -> _ = _ /\ _ = _] |- _ =>
-        apply IH in Hs; destruct Hs as [Heq1 Heq2]; try rewrite Heq1 in *;
-        try rewrite Heq2 in *; clear Heq1 Heq2
-      | Hs: stmt_reset_eval ?clsid _,
-        IH: context[stmt_reset_eval ?clsid _ -> _ = _] |- _ =>
-        apply IH in Hs; try rewrite Hs in *; clear Hs
-      | Hs: stmt_eval ?menv ?env ?stmt _,
-        IH: context[stmt_eval ?menv ?env ?stmt _ -> (_, _) = _] |- _ =>
-        apply IH in Hs; injection Hs; intros Heq1 Heq2;
-        try rewrite Heq1 in *; try rewrite Heq2 in *; clear Heq1 Heq2 Hs
-      | H1: add_obj ?o ?omenv ?menv = ?menv1,
-        H2: add_obj ?o ?omenv ?menv = ?menv2 |- _ =>
-        rewrite H1 in H2; rewrite H2 in *; clear H1 H2
-      | _ => intuition
-      end.
-  Qed.
-
-End stmt_eval.
+Lemma stmt_eval_det:
+  forall prog s menv env renv1 renv2,
+    stmt_eval prog menv env s renv1
+    -> stmt_eval prog menv env s renv2
+    -> renv1 = renv2.
+Proof.
+  intros prog s menv env renv1 renv2 Hs1.
+  revert renv2.
+  induction Hs1 using stmt_eval_mult
+  with (P:=fun prog menv env s renv1 sev=>
+             forall renv2, stmt_eval prog menv env s renv2 -> renv1 = renv2)
+       (P0:=fun prog menv clsid v menv' rv ssev=>
+              forall menv'' rv', stmt_step_eval prog menv clsid v menv'' rv'
+                                 -> menv' = menv'' /\ rv = rv')
+       (P1:=fun prog i menv srev=>
+              forall menv', stmt_reset_eval prog i menv' -> menv = menv');
+    inversion_clear 1;
+    repeat progress match goal with
+    | Ht: exp_eval ?menv ?env ?e (Cbool true),
+      Hf: exp_eval ?menv ?env ?e (Cbool false) |- _ =>
+      pose proof (exp_eval_det _ _ _ _ _ Ht Hf) as Hneq; discriminate
+    | H1:exp_eval ?menv ?env ?e ?v1,
+      H2:exp_eval ?menv ?env ?e ?v2 |- _ =>
+      pose proof (exp_eval_det _ _ _ _ _ H1 H2) as Heq;
+        rewrite Heq in *; clear Heq H1 H2
+    | H1: PM.add ?x ?v ?env = ?env1,
+      H2: PM.add ?x ?v ?env = ?env2 |- _ =>
+      rewrite H1 in H2; rewrite H2 in *; clear H1 H2
+    | H1: add_mem ?x ?v ?menv = ?menv1,
+      H2: add_mem ?x ?v ?menv = ?menv2 |- _ =>
+      rewrite H1 in H2; rewrite H2 in *; clear H1 H2
+    | H1: find_obj ?o ?menv = Some ?omenv1,
+      H2: find_obj ?o ?menv = Some ?omenv2 |- _ =>
+      rewrite H1 in H2; injection H2; intro Heq; rewrite Heq in *;
+      clear H1 H2 Heq
+    | H1: find_class ?clsid ?prog = _,
+      H2: find_class ?clsid ?prog = _ |- _ =>
+      rewrite H1 in H2; injection H2;
+      intros Heq1 Heq2; rewrite Heq1, Heq2 in *; clear H2 H2 Heq1 Heq2
+    | H1: PM.find ?x ?env = ?rv1,
+      H2: PM.find ?x ?env = ?rv2 |- _ =>
+      rewrite H1 in H2; injection H2; rewrite H2 in *; clear H1 H2
+    | Hs: stmt_step_eval ?prog ?omenv ?clsid ?v _ _,
+          IH: context[stmt_step_eval ?prog ?omenv ?clsid ?v _ _ -> _ = _ /\ _ = _]
+              |- _ =>
+      apply IH in Hs; destruct Hs as [Heq1 Heq2]; try rewrite Heq1 in *;
+      try rewrite Heq2 in *; clear Heq1 Heq2
+    | Hs: stmt_reset_eval ?prog ?clsid _,
+      IH: context[stmt_reset_eval ?prog ?clsid _ -> _ = _] |- _ =>
+      apply IH in Hs; try rewrite Hs in *; clear Hs
+    | Hs: stmt_eval ?prog ?menv ?env ?stmt _,
+      IH: context[stmt_eval ?prog ?menv ?env ?stmt _ -> (_, _) = _] |- _ =>
+      apply IH in Hs; injection Hs; intros Heq1 Heq2;
+      try rewrite Heq1 in *; try rewrite Heq2 in *; clear Heq1 Heq2 Hs
+    | H1: add_obj ?o ?omenv ?menv = ?menv1,
+      H2: add_obj ?o ?omenv ?menv = ?menv2 |- _ =>
+      rewrite H1 in H2; rewrite H2 in *; clear H1 H2
+    | _ => intuition
+    end.
+Qed.
 
 Lemma find_mem_gss:
   forall y c m, find_mem y (add_mem y c m) = Some c.
